theories/typing_prop.v
@@ -371,198 +371,198 @@ Proof.
   - eauto with wff.
 Qed.
 
-Lemma regularity Γ a A : Γ ⊢ a ∈ A -> exists i, Γ ⊢ A ∈ tUniv i.
-Proof.
-  move => h.
-  elim : Γ a A / h.
-  - admit.
-  - sfirstorder ctrs:Wt.
-  - sfirstorder.
-  - move => Γ a A B b ha [i hPi] hb [j hA].
-    move /Wt_Pi_inv : hPi => [k][hk]hk'.
-    exists k. move : subst_wt hb hk'. repeat move /[apply]. apply.
-  - admit.
-  - qauto l:on ctrs:Wt.
-Admitted.
+(* Lemma regularity Γ a A : Γ ⊢ a ∈ A -> exists i, Γ ⊢ A ∈ tUniv i. *)
+(* Proof. *)
+(*   move => h. *)
+(*   elim : Γ a A / h. *)
+(*   - admit. *)
+(*   - sfirstorder ctrs:Wt. *)
+(*   - sfirstorder. *)
+(*   - move => Γ a A B b ha [i hPi] hb [j hA]. *)
+(*     move /Wt_Pi_inv : hPi => [k][hk]hk'. *)
+(*     exists k. move : subst_wt hb hk'. repeat move /[apply]. apply. *)
+(*   - *)
+(*   - qauto l:on ctrs:Wt. *)
+(* Admitted. *)
 
-Lemma Equiv_Wt Γ a b A : Γ ⊢ a ≡ b ∈ A -> Γ ⊢ a ∈ A /\ Γ ⊢ b ∈ A.
-Proof.
-  move => h. elim : Γ a b A / h.
-  - hauto lq:on ctrs:Wt.
-  - sfirstorder.
-  - sfirstorder.
-  - move => Γ i A0 B0 A1 B1 h0 [ih00 ih01] h1 [ih10 ih11] h.
-    split. hauto lq:on ctrs:Equiv, Wt.
-    apply T_Pi => //.
-    move /(morphing_wt var_tm (A1 :: Γ)) : ih11. asimpl.
-    apply; last by eauto with wff.
-    rewrite /subst_ok.
-    inversion 1; subst; asimpl.
-    eapply T_Conv with (A := A1 ⟨S⟩) (i := i); eauto.
-    hauto lq:on ctrs:Wt,lookup db:wff.
-    apply E_Sym. change (tUniv i) with (tUniv i)⟨S⟩.
-    by apply : weakening_equiv; eauto with wff.
-    change (var_tm (S n)) with (var_tm n)⟨S⟩.
-    apply weakening_wt with (i := i)=>//.
-    hauto lq:on ctrs:Wt db:wff.
-  - move => Γ A0 A1 a0 a1 B i hA [ihA0 ihA1] h0 hPi hPi' ha [iha0 iha1].
-    split.
-    hauto lq:on ctrs:Wt.
-    apply T_Conv with (A := tPi A1 B) (i := i).
-    apply : T_Abs; eauto.
-    (* morphing context *)
-    sfirstorder use: ctx_morph.
-    hauto lq:on ctrs:Equiv.
-  - move => Γ a0 b0 a1 b1 A B hb [ihb0 ihb1]ha [iha0 iha1].
-    split; first by eauto using T_App.
-    (* Use regularity *)
-    (* apply T_Conv with (A := B[a1..]) (i := i); *)
-    (*   first by eauto using T_App. *)
-    (* Need cong2 *)
-    admit.
-  - move => Γ A B a b i hT hb ha.
-    move /Wt_Pi_inv : (hT) => [j][h0]h1.
-    split.
-    + eapply T_App; eauto.
-      apply : T_Abs; eauto.
-    + eauto using subst_wt.
-  - hauto lq:on ctrs:Wt.
-  - hauto lq:on ctrs:Wt.
-Admitted.
+(* Lemma Equiv_Wt Γ a b A : Γ ⊢ a ≡ b ∈ A -> Γ ⊢ a ∈ A /\ Γ ⊢ b ∈ A. *)
+(* Proof. *)
+(*   move => h. elim : Γ a b A / h. *)
+(*   - hauto lq:on ctrs:Wt. *)
+(*   - sfirstorder. *)
+(*   - sfirstorder. *)
+(*   - move => Γ i A0 B0 A1 B1 h0 [ih00 ih01] h1 [ih10 ih11] h. *)
+(*     split. hauto lq:on ctrs:Equiv, Wt. *)
+(*     apply T_Pi => //. *)
+(*     move /(morphing_wt var_tm (A1 :: Γ)) : ih11. asimpl. *)
+(*     apply; last by eauto with wff. *)
+(*     rewrite /subst_ok. *)
+(*     inversion 1; subst; asimpl. *)
+(*     eapply T_Conv with (A := A1 ⟨S⟩) (i := i); eauto. *)
+(*     hauto lq:on ctrs:Wt,lookup db:wff. *)
+(*     apply E_Sym. change (tUniv i) with (tUniv i)⟨S⟩. *)
+(*     by apply : weakening_equiv; eauto with wff. *)
+(*     change (var_tm (S n)) with (var_tm n)⟨S⟩. *)
+(*     apply weakening_wt with (i := i)=>//. *)
+(*     hauto lq:on ctrs:Wt db:wff. *)
+(*   - move => Γ A0 A1 a0 a1 B i hA [ihA0 ihA1] h0 hPi hPi' ha [iha0 iha1]. *)
+(*     split. *)
+(*     hauto lq:on ctrs:Wt. *)
+(*     apply T_Conv with (A := tPi A1 B) (i := i). *)
+(*     apply : T_Abs; eauto. *)
+(*     (* morphing context *) *)
+(*     sfirstorder use: ctx_morph. *)
+(*     hauto lq:on ctrs:Equiv. *)
+(*   - move => Γ a0 b0 a1 b1 A B hb [ihb0 ihb1]ha [iha0 iha1]. *)
+(*     split; first by eauto using T_App. *)
+(*     (* Use regularity *) *)
+(*     (* apply T_Conv with (A := B[a1..]) (i := i); *) *)
+(*     (*   first by eauto using T_App. *) *)
+(*     (* Need cong2 *) *)
+(*     admit. *)
+(*   - move => Γ A B a b i hT hb ha. *)
+(*     move /Wt_Pi_inv : (hT) => [j][h0]h1. *)
+(*     split. *)
+(*     + eapply T_App; eauto. *)
+(*       apply : T_Abs; eauto. *)
+(*     + eauto using subst_wt. *)
+(*   - hauto lq:on ctrs:Wt. *)
+(*   - hauto lq:on ctrs:Wt. *)
+(* Admitted. *)
 
-Definition subst2_ok ρ0 ρ1 Γ Δ :=
-  forall i A, lookup i Γ A -> Δ ⊢ ρ0 i ≡ ρ1 i ∈ A [ ρ0 ].
+(* Definition subst2_ok ρ0 ρ1 Γ Δ := *)
+(*   forall i A, lookup i Γ A -> Δ ⊢ ρ0 i ≡ ρ1 i ∈ A [ ρ0 ]. *)
 
-Lemma subst2_lrefl ρ0 ρ1 Γ Δ :
-  subst2_ok ρ0 ρ1 Γ Δ -> subst_ok ρ0 Γ Δ.
-Proof.
-  hauto lq:on use:Wt_Equiv, Equiv_Wt unfold:subst2_ok, subst_ok.
-Qed.
+(* Lemma subst2_lrefl ρ0 ρ1 Γ Δ : *)
+(*   subst2_ok ρ0 ρ1 Γ Δ -> subst_ok ρ0 Γ Δ. *)
+(* Proof. *)
+(*   hauto lq:on use:Wt_Equiv, Equiv_Wt unfold:subst2_ok, subst_ok. *)
+(* Qed. *)
 
-Lemma subst2_up ρ0 ρ1 k Γ Δ A
-  (h : subst2_ok ρ0 ρ1 Γ Δ) :
-  Δ ⊢ A[ρ0] ∈ tUniv k ->
-  subst2_ok (up_tm_tm ρ0) (up_tm_tm ρ1) (A :: Γ) (A[ρ0] :: Δ).
-Proof.
-  rewrite /subst2_ok => h0 i A0.
-  elim /lookup_inv_cons. asimpl.
-  have -> : A[ρ0 >> ren_tm S] = A[ρ0]⟨S⟩ by asimpl.
-  apply E_Var.
-  hauto lq:on db:wff.
-  by constructor.
-  move => j B ? ? ?. subst.
-  asimpl.
-  have -> : B[ρ0 >> ren_tm S] = B[ρ0]⟨S⟩ by asimpl.
-  apply weakening_equiv with (i := k)=>//.
-  by apply h.
-Qed.
+(* Lemma subst2_up ρ0 ρ1 k Γ Δ A *)
+(*   (h : subst2_ok ρ0 ρ1 Γ Δ) : *)
+(*   Δ ⊢ A[ρ0] ∈ tUniv k -> *)
+(*   subst2_ok (up_tm_tm ρ0) (up_tm_tm ρ1) (A :: Γ) (A[ρ0] :: Δ). *)
+(* Proof. *)
+(*   rewrite /subst2_ok => h0 i A0. *)
+(*   elim /lookup_inv_cons. asimpl. *)
+(*   have -> : A[ρ0 >> ren_tm S] = A[ρ0]⟨S⟩ by asimpl. *)
+(*   apply E_Var. *)
+(*   hauto lq:on db:wff. *)
+(*   by constructor. *)
+(*   move => j B ? ? ?. subst. *)
+(*   asimpl. *)
+(*   have -> : B[ρ0 >> ren_tm S] = B[ρ0]⟨S⟩ by asimpl. *)
+(*   apply weakening_equiv with (i := k)=>//. *)
+(*   by apply h. *)
+(* Qed. *)
 
-Lemma morphing2_Syn :
-  (forall Γ a A,  Γ ⊢ a ∈ A -> forall Δ ρ0 ρ1,
-    subst2_ok ρ0 ρ1 Γ Δ ->
-    ⊢ Δ ->
-    Δ ⊢ a[ρ0] ≡ a[ρ1] ∈ A[ρ0]) /\
-  (forall Γ a b A,  Γ ⊢ a ≡ b ∈ A -> forall Δ ρ0 ρ1,
-    subst2_ok ρ0 ρ1 Γ Δ ->
-    ⊢ Δ ->
-  (* experimental version *)
-    Δ ⊢ a[ρ0] ≡ b[ρ0] ∈ A[ρ0] /\
-    Δ ⊢ a[ρ0] ≡ a[ρ1] ∈ A[ρ0] /\
-    Δ ⊢ b[ρ0] ≡ b[ρ1] ∈ A[ρ0]
+(* Lemma morphing2_Syn : *)
+(*   (forall Γ a A,  Γ ⊢ a ∈ A -> forall Δ ρ0 ρ1, *)
+(*     subst2_ok ρ0 ρ1 Γ Δ -> *)
+(*     ⊢ Δ -> *)
+(*     Δ ⊢ a[ρ0] ≡ a[ρ1] ∈ A[ρ0]) /\ *)
+(*   (forall Γ a b A,  Γ ⊢ a ≡ b ∈ A -> forall Δ ρ0 ρ1, *)
+(*     subst2_ok ρ0 ρ1 Γ Δ -> *)
+(*     ⊢ Δ -> *)
+(*   (* experimental version *) *)
+(*     Δ ⊢ a[ρ0] ≡ b[ρ0] ∈ A[ρ0] /\ *)
+(*     Δ ⊢ a[ρ0] ≡ a[ρ1] ∈ A[ρ0] /\ *)
+(*     Δ ⊢ b[ρ0] ≡ b[ρ1] ∈ A[ρ0] *)
 
-  (* the most "intuitive" def *)
-    (* Δ ⊢ a[ρ0] ≡ b[ρ1] ∈ A[ρ0] *)).
-Proof.
-  apply wt_mutual=> /=.
-  (* Var *)
-  - sfirstorder.
-  (* Pi *)
-  - move => Γ i A B hA ihA hB ihB Δ ρ0 ρ1 hρ hΔ.
-    (* have ? : Δ ⊢ A[ρ0] ∈ tUniv i by sfirstorder use:morphing_wt_univ. *)
-    apply E_Pi; eauto with wff.
-    + apply ihB=>//.
-      move => i0 A0.
-      elim /lookup_inv_cons.
-      * asimpl.
-        have -> : A[ρ0 >> ren_tm S] = A[ρ0]⟨S⟩ by asimpl.
-        apply E_Var.
-        (* Mutually proven with Equiv Wt? *)
-        (* Or adding subst_ok as premises? *)
-        (* Removable from Equiv *)
-        admit.
-        (* hauto lq:on db:wff. *)
-        by constructor.
-      * move => j B0 ? ? ?. subst. asimpl.
-        have -> : B0[ρ0 >> ren_tm S] = B0[ρ0]⟨S⟩ by asimpl.
-        apply : weakening_equiv; eauto.
-        admit.
-      * (* hauto lq:on use:morphing_wt_univ db:wff. *)
-        admit.
-    + admit.
-  (* Abs *)
-  - move => Γ A a B i hPi ihPi hA ihA ha iha Δ ρ0 ρ1 hρ hΔ.
-    move /ihPi /(_ hΔ) : (hρ) => h.
-    apply E_Abs with (i := i); eauto.
-    admit.
-    apply : E_Trans; eauto.
-    apply E_Pi.
-    admit.
-    admit.
-    admit.
-    apply iha.
-    apply : subst2_up; eauto.
-    admit.
-    admit.
-  (* App *)
-  - move => Γ a A B b i ha iha hb (* ihb hA ihA. hB ihB *) Δ ρ0 ρ1 hρ hΔ.
-    eapply E_App'; eauto. by asimpl.
-  (* Conv *)
-  - move => Γ a A B i ha iha hE ihE Δ ρ0 ρ1 hρ hΔ.
-    apply E_Conv with (A := A[ρ0]) (i := i); eauto.
-    sfirstorder use:morphing_equiv_univ.
-  (* Univ *)
-  - hauto lq:on ctrs:Equiv.
+(*   (* the most "intuitive" def *) *)
+(*     (* Δ ⊢ a[ρ0] ≡ b[ρ1] ∈ A[ρ0] *)). *)
+(* Proof. *)
+(*   apply wt_mutual=> /=. *)
+(*   (* Var *) *)
+(*   - sfirstorder. *)
+(*   (* Pi *) *)
+(*   - move => Γ i A B hA ihA hB ihB Δ ρ0 ρ1 hρ hΔ. *)
+(*     (* have ? : Δ ⊢ A[ρ0] ∈ tUniv i by sfirstorder use:morphing_wt_univ. *) *)
+(*     apply E_Pi; eauto with wff. *)
+(*     + apply ihB=>//. *)
+(*       move => i0 A0. *)
+(*       elim /lookup_inv_cons. *)
+(*       * asimpl. *)
+(*         have -> : A[ρ0 >> ren_tm S] = A[ρ0]⟨S⟩ by asimpl. *)
+(*         apply E_Var. *)
+(*         (* Mutually proven with Equiv Wt? *) *)
+(*         (* Or adding subst_ok as premises? *) *)
+(*         (* Removable from Equiv *) *)
+(*         admit. *)
+(*         (* hauto lq:on db:wff. *) *)
+(*         by constructor. *)
+(*       * move => j B0 ? ? ?. subst. asimpl. *)
+(*         have -> : B0[ρ0 >> ren_tm S] = B0[ρ0]⟨S⟩ by asimpl. *)
+(*         apply : weakening_equiv; eauto. *)
+(*         admit. *)
+(*       * (* hauto lq:on use:morphing_wt_univ db:wff. *) *)
+(*         admit. *)
+(*     + admit. *)
+(*   (* Abs *) *)
+(*   - move => Γ A a B i hPi ihPi hA ihA ha iha Δ ρ0 ρ1 hρ hΔ. *)
+(*     move /ihPi /(_ hΔ) : (hρ) => h. *)
+(*     apply E_Abs with (i := i); eauto. *)
+(*     admit. *)
+(*     apply : E_Trans; eauto. *)
+(*     apply E_Pi. *)
+(*     admit. *)
+(*     admit. *)
+(*     admit. *)
+(*     apply iha. *)
+(*     apply : subst2_up; eauto. *)
+(*     admit. *)
+(*     admit. *)
+(*   (* App *) *)
+(*   - move => Γ a A B b i ha iha hb (* ihb hA ihA. hB ihB *) Δ ρ0 ρ1 hρ hΔ. *)
+(*     eapply E_App'; eauto. by asimpl. *)
+(*   (* Conv *) *)
+(*   - move => Γ a A B i ha iha hE ihE Δ ρ0 ρ1 hρ hΔ. *)
+(*     apply E_Conv with (A := A[ρ0]) (i := i); eauto. *)
+(*     sfirstorder use:morphing_equiv_univ. *)
+(*   (* Univ *) *)
+(*   - hauto lq:on ctrs:Equiv. *)
 
-  (* Var *)
-  - hauto lq:on ctrs:Equiv, Wt unfold:subst2_ok.
+(*   (* Var *) *)
+(*   - hauto lq:on ctrs:Equiv, Wt unfold:subst2_ok. *)
 
-  (* Sym *)
-  - hauto l:on ctrs:Equiv.
+(*   (* Sym *) *)
+(*   - hauto l:on ctrs:Equiv. *)
 
-  (* Trans *)
-  - hauto l:on ctrs:Equiv.
+(*   (* Trans *) *)
+(*   - hauto l:on ctrs:Equiv. *)
 
-  (* Pi *)
-  - move => Γ i A0 B0 A1 B1 hA ihA hB ihB hA0 ihA0 Δ ρ0 ρ1 hρ hΔ.
-    repeat split.
-    apply E_Pi. hauto l:on.
-    eapply ihB. apply : subst2_up; eauto.
-    (* Need to be mutual with wt equiv *)
-    admit.
-    admit.
-    admit.
-    apply E_Pi. hauto l:on.
-    eapply ihB. apply : subst2_up; eauto.
-    admit.
-    admit.
-    admit.
-     apply E_Pi. hauto l:on.
-    eapply ihB.
-    (* Use context morph *)
-    admit.
-    admit.
-    admit.
-  (* Abs *)
-  - admit.
-  - move => Γ a0 b0 a1 b1 A B hb ihb ha iha Δ ρ0 ρ1 hρ hΔ.
-    repeat split.
-    apply : E_App';cycle 1; [hauto l:on | hauto l:on | by asimpl].
-    apply : E_App'; cycle 1; [hauto l:on | hauto l:on | by asimpl].
-    eapply E_Conv with (A := B[a1..][ρ0]).
-    apply : E_App'; cycle 1.
-    hauto l:on.
-    hauto l:on.
-    by asimpl.
+(*   (* Pi *) *)
+(*   - move => Γ i A0 B0 A1 B1 hA ihA hB ihB hA0 ihA0 Δ ρ0 ρ1 hρ hΔ. *)
+(*     repeat split. *)
+(*     apply E_Pi. hauto l:on. *)
+(*     eapply ihB. apply : subst2_up; eauto. *)
+(*     (* Need to be mutual with wt equiv *) *)
+(*     admit. *)
+(*     admit. *)
+(*     admit. *)
+(*     apply E_Pi. hauto l:on. *)
+(*     eapply ihB. apply : subst2_up; eauto. *)
+(*     admit. *)
+(*     admit. *)
+(*     admit. *)
+(*      apply E_Pi. hauto l:on. *)
+(*     eapply ihB. *)
+(*     (* Use context morph *) *)
+(*     admit. *)
+(*     admit. *)
+(*     admit. *)
+(*   (* Abs *) *)
+(*   - admit. *)
+(*   - move => Γ a0 b0 a1 b1 A B hb ihb ha iha Δ ρ0 ρ1 hρ hΔ. *)
+(*     repeat split. *)
+(*     apply : E_App';cycle 1; [hauto l:on | hauto l:on | by asimpl]. *)
+(*     apply : E_App'; cycle 1; [hauto l:on | hauto l:on | by asimpl]. *)
+(*     eapply E_Conv with (A := B[a1..][ρ0]). *)
+(*     apply : E_App'; cycle 1. *)
+(*     hauto l:on. *)
+(*     hauto l:on. *)
+(*     by asimpl. *)
 
 
 (* Admitted. *)
